src/ocaml-output/FStar_TypeChecker_DeferredImplicits.ml
@@ -704,8 +704,7 @@ let (solve_deferred_to_tactic_goals :
                                   tp.FStar_TypeChecker_Common.lhs
                                   tp.FStar_TypeChecker_Common.rhs in
                               let uu___8 =
-                                FStar_TypeChecker_Env.new_implicit_var_aux
-                                  reason
+                                FStar_TypeChecker_Env.new_implicit_var reason
                                   (tp.FStar_TypeChecker_Common.lhs).FStar_Syntax_Syntax.pos
                                   env2 goal_ty FStar_Syntax_Syntax.Strict
                                   FStar_Pervasives_Native.None in
